\documentclass{article}
 
\usepackage{tikz}
\usepackage{amsmath}
\usepackage[margin=0.75in]{geometry}
\usepackage{amssymb}
 
\title{Generalized Formalization of Game Rules}
\author{Christiaan van de Sande \and Tanner Reese}

\begin{document}

\maketitle

\section{Introduction}


\section{Rule Defenition}

$ R (A, B) = ( \lambda, \mu, \phi, \rho ) $

\subsection{The Four Functions}

\begin{align*}
  \lambda & : A \rightarrow \mathcal{P} (B) \\
      \mu & : A \times B \rightarrow B  \\
     \phi & : A \times B \rightarrow A 
\end{align*}

\begin{align*}
  \phi ( \mu (a, b), b) = b
\end{align*}

\subsection{Equivalence in $ A $ and $ B $ }

\subsection{Repeatablity of a Rule}

\subsection{Independence between Rulse}

Existence: $ \forall ~ b_R \in B_R, ~ \forall ~ b_S \in \lambda_S \circ \phi (b_R), ~ \exists ~ b'_S \in \lambda_S \circ \mu_R (b_R), b'_S \sim b''_S $ \\
Uniquenes: $ \forall ~ b_S' \in \lambda \circ \mu_R (b_R), ~ b_S' \sim  b_S'' \implies \mu_S (b_S') = \mu_S (b_S'') $

\subsection{Operations on Rules}

\subsubsection{Negation of a Repeatable Rule}

\begin{align*}
          S (A, A) & = - R (A, A) \\
  \lambda_S (a)    & = \begin{cases} \varnothing & \lambda_R (a) \neq \varnothing \\ \{ a \} & \lambda_R (a) = \varnothing \end{cases} \\
      \mu_S (a, b)    & =  \mu_R (a, b) \\
     \phi_S (a, b)    & = \phi_R (a, b) 
\end{align*}

\subsubsection{Union between Rules}

\begin{align*}
          T (A, B) & = R (A, B) \cup S (A, B) \\
  \lambda_T (a)    & = \lambda_R (a) \cup \lambda_S (a) \\
      \mu_T (a, b) & = \mu_R  (a, b)    = \mu_S  (a, b) \\
     \phi_T (a, b) & = \phi_R (a, b)    = \phi_S (a, b)
\end{align*}

\subsubsection{Intersection between Rules}

\begin{align*}
          T (A, B) & = R (A, B) \cap S (A, B) \\
  \lambda_T (a)    & = \lambda_R (a) \cap \lambda_S (a) \\
      \mu_T (a, b) & =  \mu_R (a, b) =  \mu_S (a, b) \\
     \phi_T (a, b) & = \phi_R (a, b) = \phi_S (a, b)
\end{align*}

\subsubsection{Indetpendent Product between Rules}
The independent product ($ \times $) is only defined for rules that are Independent.
\begin{align*}
          T (A, (B \times C)) & = R (A, B) \times S (A, C) \\
  \lambda_T (a)               & = \lambda_R (a) \times \lambda_S (a) \\
      \mu_T (a, (b, c))       & =  \mu_R  ( \mu_S (a, c), b) \\
     \phi_T (a, (b, c))       & = \phi_S  (\phi_R (a, b), c) 
\end{align*}

\subsubsection{Dependent Product between Rules}
The dependent product between two rules $ S \cdot R $ is only defined if $ A_S = B_R $.
\begin{align*}
          T (A, (B \times C)) & = R (A, B) \cdot S (A, B) \\
  \lambda_T (a)               & = \{ (b,c) | b \in \lambda_R (a), c \in \lambda_S (b) \} \\
      \mu_T (a, (b, c))       & =   \mu_R (a,  \mu_S (b, c)) \\
     \phi_T (a, (b, c))       & =  \phi_R (a, \phi_S (b, c)) 
\end{align*}

\subsubsection{Patterning of a Repeatable Rule over a Range}

\begin{align*}
     V (A, B)    & = R (B, B) \bigg\rvert_{S (A, B)}^{T (A, C)} \\
    \nu_V (b)    & = \begin{cases} \{ b \} & \lambda_T (b) \neq \varnothing \\ \{ b \} \cup (\widehat{\nu}_V \circ \lambda_R (x)) & \lambda_T (b) = \varnothing \end{cases} \\
\lambda_V (a)    & = \widehat{\nu}_V \circ \lambda_S (a) \\
    \mu_V (a, b) & =  \mu_S (a,  \mu_R(b, b)) \\
   \phi_V (a, b) & = \phi_S (a, \phi_R(b, b)) 
\end{align*}

\section{Implementation}

\section{Implications}

\subsection{Game Creation}

\subsection{Game Analysis}

\section{Conclusion}

\end{document}
